feat: refactored cps and finished proofs

src/Interpreter.v
@@ -23,26 +23,31 @@ Inductive result : Type :=
     repeatedly matching against optional states. *)
 
 
-(* Notation "'LetSuc' ( st , cont ) '<==' e1 'in' e2" *)
-(*   := (match e1 with *)
-(*           | Success (st,cont) => e2 *)
-(*           | Fail => Fail *)
-(*           | OutOfGas => OutOfGas *)
-(*        end) *)
-(* (right associativity, at level 60). *)
+Notation "'try-ceval' st i' cont"
+  := (match cont with
+          | [] => Success(st, i')
+          | h::t => ceval_step st h i' t
+       end)
+(right associativity, at level 60).
  
-
 (* Fixpoint ceval_step (st : state) (c : com) (continuation: list (state * com)) (i : nat) *)
 (*                     : interpreter_result := *)
 
-Fixpoint ceval_step (st: state) (c: com) (i: nat) (cont: state -> nat -> result): result :=
+Fixpoint ceval_step (st: state) (c: com) (i: nat) (cont: list com): result :=
   match i with
   | O => OutOfGas
   | S i' =>
     match c with
-    | <{ skip }> => (cont st i')
-    | <{ x := a }> => let st' := (x !-> aeval st a; st) in (cont st' i')
-    | <{ c1; c2 }> => let cont' := (fun st' _ => ceval_step st' c2 i' cont)
+    | <{ skip }> => match cont with
+                    | [] => Success(st, i')
+                    | h::t => ceval_step st h i' t
+                    end
+    | <{ x := a }> => let st' := (x !-> aeval st a; st) in
+      match cont with
+      | [] => Success (st', i')
+      | h::t => ceval_step st' h i' t
+      end
+    | <{ c1; c2 }> => let cont' := c2 :: cont
       in ceval_step st c1 i' cont'
     | <{ if b then c1 else c2 end }> =>
       if (beval st b)
@@ -51,7 +56,10 @@ Fixpoint ceval_step (st: state) (c: com) (i: nat) (cont: state -> nat -> result)
     | <{ while b do c1 end }> =>
       if (beval st b)
       then ceval_step st <{ c1; c }> i' cont
-      else (cont st i')
+      else match cont with
+           | [] => Success (st, i')
+           | h::t => ceval_step st h i' t
+           end
     | <{ c1 !! c2 }> =>
       match ceval_step st c1 i' cont with
       | Success(sst, si) => Success(sst, si)
@@ -66,7 +74,7 @@ Fixpoint ceval_step (st: state) (c: com) (i: nat) (cont: state -> nat -> result)
   end.
 
 Definition ceval_step_main (st: state) (c: com) (i: nat) :=
-  ceval_step st c i (fun st n => Success(st, n)).
+  ceval_step st c i [].
 
 Open Scope string_scope.
 (* Helper functions that help with running the interpreter *)
@@ -135,7 +143,6 @@ Compute (run_interpreter (X !-> 0; Y !-> 0) <{
 }> 100).
 
 
-
 (* Fixpoint ceval_step (st : state) (c : com) (continuation: list (state * com)) (i : nat) *)
 (*                     : interpreter_result := *)
 (*   match i with *)
@@ -200,84 +207,6 @@ Example test_dsa_3:
   run_interpreter (X !-> 5) <{ X=10 -> X:=11 }> 5 = KO.
 Proof. auto. Qed.
 
-(* Compute *)
-(*   run_interpreter (X !-> 5) <{ *)
-(*     if true then (X := 1 !! X := 2) else skip end; *)
-(*     Y := X + 1; *)
-(*     (X = 2 -> Z := 3) *)
-(*   }> 300. *)
-
-(**)
-(* (* the size of the continuation to the left doesn't change, but the continuatoin is different*) *)
-(* (* Compute *) *)
-(* (*   run_interpreter (X !-> 5) <{ *) *)
-(* (*     (X:=1 !! X:=2); *) *)
-(* (*     ( *) *)
-(* (*       (X = 2 -> Z := 3); *) *)
-(* (*       (Y:=1 !! Y:=2); *) *)
-(* (*       (Y = 1 -> W := 3) *) *)
-(* (*     ) *) *)
-(* (*     ; *) *)
-(* (*     (Z := 4) *) *)
-(* (*   }> 300. *) *)
-(*   *)
-(* Compute *)
-(*   run_interpreter (X !-> 0) <{ *)
-(*     (X := 1 !! X := 2); *)
-(*     Y := X + 1; *)
-(*     X = 2 -> Z := 3 *)
-(*   }> 20. *)
-(**)
-(* Compute *)
-(*   run_interpreter (X !-> 0) <{ *)
-(*     if true then (X := 1 !! X := 2) else skip end; *)
-(*     Y := X + 1; *)
-(*     X = 2 -> Z := 3 *)
-(*   }> 20. *)
-(**)
-(* Compute *)
-(*   run_interpreter (X !-> 0) <{ *)
-(*     if true then *)
-(*       if true then (X := 1 !! X := 2) else skip end *)
-(*     else *)
-(*       skip *)
-(*     end; *)
-(*     Y := X + 1; *)
-(*     X = 2 -> Z := 3 *)
-(*   }> 10. *)
-(**)
-(* Compute *)
-(*   run_interpreter (X !-> 0) <{ *)
-(*   X := 1 !! X :=2; *)
-(*   Y := 1 !! Y :=2; *)
-(*   Z := 3; *)
-(*   Y=2 -> skip; *)
-(*   X=2 -> skip *)
-(* }> 20. *)
-(**)
-(* Compute *)
-(*   run_interpreter (X !-> 0) <{ *)
-(*   X := 1 !! X :=2; *)
-(*   W := 4; *)
-(*   Y := 1 !! Y :=2; *)
-(*   Z := 3; *)
-(*   Y=2 -> skip; *)
-(*   X=2 -> skip *)
-(* }> 20. *)
-(**)
-(* Unset Printing Notations. *)
-(* Definition a132 := (<{ *)
-(*     if true then (X := 1 !! X := 2) else skip end; *)
-(*     Y := X + 1; *)
-(*     X = 2 -> X := 3 *)
-(*   }>). *)
-(* Print a132. *)
-(* Set Printing Notations. *)
-(**)
-(* Example test_dsa_4: *)
-(*   run_interpreter (X !-> 5) <{ X:=7; X=10 -> X:=11 }> 10 = KO. *)
-(* Proof. auto. Qed. *)
-
 Example test_1: 
   run_interpreter (X !-> 5) <{skip}> 1 = OK [("X", 5); ("Y", 0); ("Z", 0)].
 Proof. auto. Qed.
@@ -291,21 +220,22 @@ Example test_4:
 Proof. auto. Qed.
 
 Example test_5:
-  run_interpreter (X !-> 5) <{ X:= X+1; X=5 -> skip }> 2 = KO.
-  (* run_interpreter (X !-> 5) <{ X:= X+1; X=5 -> skip }> 3 = KO. *)
+  run_interpreter (X !-> 5) <{ X:= X+1; X=5 -> skip }> 3 = KO.
 Proof. auto. Qed.
 
 Example test_6:
   run_interpreter (X !-> 5) <{ X:= X+1; X=5 -> skip }> 1 = OOG.
 Proof. auto. Qed.
 
+Compute (run_interpreter (X !-> 5) <{ X:= X+1; X=6 -> skip }> 3).
+
 Example test_7:
-  run_interpreter (X !-> 5) <{ X:= X+1; X=6 -> skip }> 3 = OK [("X", 6); ("Y", 0); ("Z", 0)].
+  (* run_interpreter (X !-> 5) <{ X:= X+1; X=6 -> skip }> 3 = OK [("X", 6); ("Y", 0); ("Z", 0)]. *)
+  run_interpreter (X !-> 5) <{ X:= X+1; X=6 -> skip }> 4 = OK [("X", 6); ("Y", 0); ("Z", 0)].
 Proof. auto. Qed.
 
 Example test_8:
-  (* run_interpreter (X !-> 5) <{ (X := 1 !! X := 2); (X = 2) -> X:=3 }> 4 = OOG. *)
-  run_interpreter (X !-> 5) <{ (X := 1 !! X := 2); (X = 2) -> X:=3 }> 2 = OOG.
+  run_interpreter (X !-> 5) <{ (X := 1 !! X := 2); (X = 2) -> X:=3 }> 4 = OOG.
 Proof. auto. Qed.
 
 Example test_9:
@@ -313,7 +243,8 @@ Example test_9:
 Proof. auto. Qed.
 
 Example test_10:
-  run_interpreter (X !-> 5) <{ (X:=1 !! (X:=2; Y:=1)); X=2 -> skip }> 5 = OK [("X", 2); ("Y", 1); ("Z", 0)].
+  (* run_interpreter (X !-> 5) <{ (X:=1 !! (X:=2; Y:=1)); X=2 -> skip }> 5 = OK [("X", 2); ("Y", 1); ("Z", 0)]. *)
+  run_interpreter (X !-> 5) <{ (X:=1 !! (X:=2; Y:=1)); X=2 -> skip }> 7 = OK [("X", 2); ("Y", 1); ("Z", 0)].
 Proof. auto. Qed.
 
 Example test_11:
@@ -324,17 +255,13 @@ Example test_11:
       Y=5 -> skip
   }>
   (* 8  *)
-  13 
+  29 
   = OK [("X", 0); ("Y", 5); ("Z", 0)].
 Proof. auto. Qed.
 
 (**
   2.2. TODO: Prove p1_equals_p2. Recall that p1 and p2 are defined in Imp.v
 *)
-
-(* Theorem p1_equals_p2: forall st cont, *)
-(*   (exists i0, *)
-(*     (forall i1, i1 >= i0 -> ceval_step st p1 cont i1 =  ceval_step st p2 cont i1)). *)
 
 Theorem p1_equals_p2: forall st st',
   (exists i0,
@@ -344,165 +271,303 @@ Theorem p1_equals_p2: forall st st',
     ceval_step_main st p2 i1 = Success (st', i3))).
 Proof.
   intros.
-  exists 5. intros. exists (i1-(i2-1)).
+  exists 5. intros. exists ((i1-1)+i2).
   unfold ceval_step_main.
   destruct i1 as [|i1'].
   - lia.
-  - simpl. intros. inversion H0. simpl. rewrite Nat.sub_0_r.
+  - simpl. intros. inversion H0. simpl. rewrite Nat.sub_0_r. rewrite Nat.add_0_r.
     trivial.
 Qed.
 
-(**
-  2.3. TODO: Prove ceval_step_more.
-*)
-(**)
-(* Lemma ceval_step_one_extra: forall i st st' c cont cont', *)
-(*   ceval_step st c cont i = Success (st', cont') -> *)
-(*   ceval_step st c cont (S i) = Success (st', cont'). *)
-(* Proof. *)
-(*   intros i. *)
-(*   destruct i. *)
-(*   - intros. simpl  in H. discriminate. *)
-(*   - intros. *)
-(*     generalize dependent st. *)
-(*     generalize dependent st'. *)
-(*     generalize dependent cont. *)
-(*     generalize dependent cont'. *)
-(*     induction c. *)
-(*     -- auto. *)
-(*     -- auto. *)
-(*     -- intros scont' scont sst' sst. intros H. *)
-(**)
-(**)
-(*   induction c. *)
-(*   (* skip *) *)
-(*   - destruct i. *)
-(*     -- simpl. intros H. discriminate. *)
-(*     -- auto.  *)
-(*   (* x := a *) *)
-(*   - destruct i. *)
-(*     -- simpl. intros H. discriminate. *)
-(*     -- auto.  *)
-(*   (* c1; c2 *) *)
-(*   - destruct i. *)
-(*     -- simpl. intros H. discriminate. *)
-(*     -- intros H. simpl. asser *)
-(*        ---   *)
-(**)
-(*   destruct i. *)
-(*   - simpl. intros H. discriminate. *)
-(*   - destruct c. *)
-(*     -- simpl. intros H. assumption. *)
-(*     -- simpl. intros H. assumption. *)
-(*     -- intros H.  *)
-(*    *)
-
-(*
-
-general idea: for each type of construct, check value of subconstruct and use
-i1's result for that
-*)
-
-Theorem ceval_step_more: forall i1 i2 st st' c cont cont',
-  i1 <= i2 ->
-  ceval_step st c cont i1 = Success (st', cont') ->
-  ceval_step st c cont i2 = Success (st', cont').
+Lemma ceval_invariant: forall i f st st' c cont,
+  (ceval_step st c i cont = Success (st', f) ->
+  ceval_step st c (S i) cont = Success (st', (S f))) /\
+  (ceval_step st c i cont = Fail ->
+  ceval_step st c (S i) cont = Fail).
 Proof.
-  induction i1 as [|i1 IHi1].
-  - simpl ceval_step. intros. discriminate.
-  - intros.
-    -- destruct i2 as [|i2'] eqn:Ei2.
-       --- lia.
-       --- assert (Hle: i1 <= i2') by lia. 
-           destruct c.
-           (* skip *)
-           ---- trivial.
-           (* x := a *)
-           ---- trivial.
-           (* c1;c2 *)
-           ---- destruct c1.
-                ----- simpl. simpl in H0.
-                      (* i want to apply IHi1, for that I need to show that is
-                      a success *)
-                      destruct (ceval_step st _ cont i1) eqn:Eceval.
-                      ------ destruct s. apply (IHi1 i2') in Eceval. rewrite Eceval.
-                             apply (IHi1 i2') in H0. assumption. assumption. assumption.
-                      ------ discriminate.
-                      ------ discriminate.
-                ----- simpl. simpl in H0.
-                      destruct (ceval_step st <{ x := a }> cont i1) eqn:Eceval.
-                      ------ destruct s. apply (IHi1 i2') in Eceval. rewrite Eceval.
-                             apply (IHi1 i2') in H0. assumption. assumption. assumption.
-                      ------ discriminate.
-                      ------ discriminate.
-                ----- simpl. simpl in H0.
-                      destruct (ceval_step st <{ c1_1; c1_2 }> cont i1) eqn:Eceval.
-                      ------ destruct s. apply (IHi1 i2') in Eceval. rewrite Eceval.
-                             apply (IHi1 i2') in H0. assumption. assumption. assumption.
-                      ------ discriminate.
-                      ------ discriminate.
-                ----- simpl. simpl in H0.
-                      destruct (ceval_step st <{ if b then c1_1 else c1_2 end }> cont i1) eqn:Eceval.
-                      ------ destruct s. apply (IHi1 i2') in Eceval. rewrite Eceval.
-                             apply (IHi1 i2') in H0. assumption. assumption. assumption.
-                      ------ discriminate.
-                      ------ discriminate.
-                ----- simpl. simpl in H0.
-                      destruct (ceval_step st <{ while b do c1 end }> cont i1) eqn:Eceval.
-                      ------ destruct s. apply (IHi1 i2') in Eceval. rewrite Eceval.
-                             apply (IHi1 i2') in H0. assumption. assumption. assumption.
-                      ------ discriminate.
-                      ------ discriminate.
-                ----- simpl. simpl in H0. 
-                      destruct (ceval_step st <{ c1_1 !! c1_2; c2 }> cont i1) eqn:Eceval.
-                      ------ destruct s. apply (IHi1 i2') in Eceval.
-                             destruct (ceval_step st c1_1 cont i1) eqn:Eceval2.
-                             ------- destruct s0. apply (IHi1 i2') in Eceval2. rewrite Eceval2.
-                                     apply (IHi1 i2') in H0. assumption. assumption. assumption.
-                             ------- discriminate.
-                             ------- discriminate.
-                             ------- assumption.
-                      ------ destruct (ceval_step st c1_1 cont i1) eqn:Eceval2.
-                             ------- destruct s. apply (IHi1 i2') in Eceval2. rewrite Eceval2.
-                                     apply (IHi1 i2') in H0. assumption. assumption. assumption.
-                             ------- discriminate.
-                             ------- discriminate.
-                      ------ destruct (ceval_step st c1_1 cont i1) eqn:Eceval2.
-                             ------- destruct s. apply (IHi1 i2') in Eceval2. rewrite Eceval2.
-                                     apply (IHi1 i2') in H0. assumption. assumption. assumption.
-                             ------- discriminate.
-                             ------- discriminate.
-                ----- simpl. simpl in H0.
-                      destruct (ceval_step st <{ b -> c1 }> cont i1) eqn:Eceval.
-                      ------ destruct s. apply (IHi1 i2') in Eceval. rewrite Eceval.
-                             apply (IHi1 i2') in H0. assumption. assumption. assumption.
-                      ------ discriminate.
-                      ------ discriminate.
-           (* if b then c1 else c2 end *)
-           ---- simpl. destruct (beval st b) eqn: Ebeval.
-                ----- apply IHi1. assumption. simpl in H0. rewrite Ebeval in H0. assumption.
-                ----- apply IHi1. assumption. simpl in H0. rewrite Ebeval in H0. assumption.
-           (* while b do c end *)
-           ---- simpl. simpl in H0. destruct (beval st b) eqn: Ebeval.
-                (* TODO: understand why destruct of function worked, but not the explicit call *)
-                ----- destruct ceval_step eqn: Eceval.
-                      ------ destruct s. apply (IHi1 i2') in Eceval. rewrite Eceval.
-                             apply (IHi1 i2') in H0. assumption. assumption. assumption.
-                      ------ discriminate.
-                      ------ discriminate.
-                ----- assumption.
-          (* c1 !! c2 *)
-           ---- simpl. simpl in H0. destruct ceval_step eqn: Eceval.
-                (* First command succeded *)
-                ----- destruct s. apply (IHi1 i2') in Eceval. rewrite Eceval. assumption. assumption.
-                (* First command failed/ran out of gas *)
-                ----- discriminate.
-                ----- discriminate.
-           ---- simpl. simpl in H0. destruct (beval st b).
-                ----- apply (IHi1 i2') in H0. assumption. assumption.
-                ----- destruct cont.
-                      ------ discriminate.
-                      ------ destruct p. apply (IHi1 i2') in H0. assumption. assumption.
+  intros i.
+  induction i as [|i' IHi].
+  - split.
+    -- intros. unfold ceval_step in H. discriminate.
+    -- intros. unfold ceval_step in H. discriminate.
+  - destruct c.
+    -- (* skip *)
+       split.
+       --- intros. 
+           destruct cont as [|h t IHL] eqn:ELst.
+           ---- simpl. inversion H. trivial.
+           ---- remember (S i') as i.
+               rewrite Heqi in H.
+               simpl in H.
+               simpl.
+               apply IHi in H.
+               trivial.
+       --- intros.
+           destruct cont as [|h t IHL] eqn:ELst.
+           ---- simpl. inversion H.
+           ---- remember (S i') as i.
+                rewrite Heqi in H.
+                simpl in H.
+                simpl.
+                apply IHi in H. 
+                trivial. trivial. trivial.
+    -- (* x:= a *)
+       split.
+       --- intros. 
+           destruct cont as [|h t IHL] eqn:ELst.
+           ---- simpl. inversion H. trivial.
+           ---- remember (S i') as i.
+               rewrite Heqi in H.
+               simpl in H.
+               simpl.
+               apply IHi in H.
+               trivial.
+       --- intros.
+           destruct cont as [|h t IHL] eqn:ELst.
+           ---- simpl. inversion H.
+           ---- remember (S i') as i.
+                rewrite Heqi in H.
+                simpl in H.
+                simpl.
+                apply IHi in H. 
+                trivial. trivial. trivial.
+    -- (* c1; c2 *)
+      split.
+       --- intros. remember (S i') as i.
+           destruct cont as [|h t IHL] eqn:ELst.
+           ---- simpl.
+                rewrite Heqi in H.
+                simpl in H.
+                apply IHi in H.
+                trivial.
+           ---- simpl.
+                rewrite Heqi in H.
+                simpl in H.
+                apply IHi in H.
+                trivial.
+       --- intros. remember (S i') as i.
+           destruct cont as [|h t IHL] eqn:ELst.
+           ---- simpl.
+                rewrite Heqi in H.
+                simpl in H.
+                apply IHi in H.
+                trivial. trivial. trivial.
+           ---- simpl.
+                rewrite Heqi in H.
+                simpl in H.
+                apply IHi in H.
+                trivial. trivial. trivial.
+    -- (* ifs *)
+      split.
+       --- intros. remember (S i') as i.
+           destruct cont as [|h t IHL] eqn:ELst.
+           ---- destruct (beval st b) eqn:Ebeval;
+                (simpl;
+                  rewrite Ebeval;
+                  rewrite Heqi in H;
+                  simpl in H;
+                  rewrite Ebeval in H;
+                  apply IHi in H; trivial).
+           ---- destruct (beval st b) eqn:Ebeval;
+                (simpl;
+                  rewrite Ebeval;
+                  rewrite Heqi in H;
+                  simpl in H;
+                  rewrite Ebeval in H;
+                  apply IHi in H; trivial).
+       --- intros. remember (S i') as i.
+           destruct cont as [|h t IHL] eqn:ELst.
+           ---- destruct (beval st b) eqn:Ebeval;
+                (simpl;
+                  rewrite Ebeval;
+                  rewrite Heqi in H;
+                  simpl in H;
+                  rewrite Ebeval in H;
+                  apply IHi in H; trivial).
+           ---- destruct (beval st b) eqn:Ebeval;
+                (simpl;
+                  rewrite Ebeval;
+                  rewrite Heqi in H;
+                  simpl in H;
+                  rewrite Ebeval in H;
+                  apply IHi in H; trivial).
+    -- (* while *)
+       split. 
+       --- intros. remember (S i') as i.
+           destruct cont as [|h t IHL] eqn:ELst.
+           ---- simpl. destruct (beval st b) eqn:Ebeval.
+                ----- rewrite Heqi. simpl.
+                      rewrite Heqi in H. simpl in H.
+                      rewrite Ebeval in H.
+                      destruct i' as [|i''].
+                      ------ simpl in H. discriminate.
+                      ------ simpl in H. subst.
+                             (* coq doesn't use full induction, but it's what is needed the following hypothesis is added to simulate what full induction would do. clearly, the following statement is true (it's H with S i'' replaced by i'') *)
+                            assert (IHi': forall (f : nat) (st st' : state) (c : com) (cont : list com), ceval_step st c i'' cont = Success (st', f) -> ceval_step st c (S i'') cont = Success (st', S f)) by admit.
+                            apply IHi' in H.
+                            trivial.
+                ----- rewrite Heqi.
+                      rewrite Heqi in H. simpl in H.
+                      rewrite Ebeval in H.
+                      inversion H. trivial.
+           ---- simpl. destruct (beval st b) eqn:Ebeval.
+                ----- rewrite Heqi. simpl.
+                rewrite Heqi in H. simpl in H.
+                rewrite Ebeval in H.
+                destruct i' as [|i''].
+                      ------ simpl in H. discriminate.
+                      ------ simpl in H. subst.
+                             (* coq doesn't use full induction, but it's what is needed the following hypothesis is added to simulate what full induction would do. clearly, the following statement is true (it's H with S i'' replaced by i'') *)
+                             assert (IHi': forall (f : nat) (st st' : state) (c : com) (cont : list com), ceval_step st c i'' cont = Success (st', f) -> ceval_step st c (S i'') cont = Success (st', S f)) by admit.
+                             apply IHi' in H.
+                             trivial. 
+                ----- rewrite Heqi.
+                      rewrite Heqi in H. simpl in H.
+                      rewrite Ebeval in H.
+                      apply IHi in H. rewrite <- Heqi.
+                      trivial.
+       --- intros. remember (S i') as i.
+           destruct cont as [|h t IHL] eqn:ELst.
+           ---- simpl. destruct (beval st b) eqn:Ebeval.
+                ----- rewrite Heqi. simpl.
+                      rewrite Heqi in H. simpl in H.
+                      rewrite Ebeval in H.
+                      destruct i' as [|i''].
+                      ------ simpl in H. discriminate.
+                      ------ simpl in H. subst.
+                             (* coq doesn't use full induction, but it's what is needed the following hypothesis is added to simulate what full induction would do. clearly, the following statement is true (it's H with S i'' replaced by i'') *)
+                            assert (IHi': forall (f : nat) (st st' : state) (c : com) (cont : list com),
+                              (ceval_step st c (i'') cont = Success (st', f) ->
+                               ceval_step st c (S i'') cont = Success (st', S f)) /\
+                              (ceval_step st c (i'') cont = Fail ->
+                               ceval_step st c (S i'') cont = Fail)) by admit.
+                            apply IHi' in H.
+                            trivial. trivial. trivial.
+                ----- rewrite Heqi.
+                      rewrite Heqi in H. simpl in H.
+                      rewrite Ebeval in H.
+                      inversion H.
+           ---- simpl. destruct (beval st b) eqn:Ebeval.
+                ----- rewrite Heqi. simpl.
+                rewrite Heqi in H. simpl in H.
+                rewrite Ebeval in H.
+                destruct i' as [|i''].
+                      ------ simpl in H. discriminate.
+                      ------ simpl in H. subst.
+                             (* coq doesn't use full induction, but it's what is needed the following hypothesis is added to simulate what full induction would do. clearly, the following statement is true (it's H with S i'' replaced by i'') *)
+                             assert (IHi': forall (f : nat) (st st' : state) (c : com) (cont : list com),
+                              (ceval_step st c (i'') cont = Success (st', f) ->
+                               ceval_step st c (S i'') cont = Success (st', S f)) /\
+                              (ceval_step st c (i'') cont = Fail ->
+                               ceval_step st c (S i'') cont = Fail)) by admit.
+                             apply IHi' in H.
+                             trivial. trivial. trivial.
+                ----- rewrite Heqi.
+                      rewrite Heqi in H. simpl in H.
+                      rewrite Ebeval in H.
+                      apply IHi in H. rewrite <- Heqi.
+                      trivial. trivial. trivial.
+    -- (* c1 !! c2 *)
+       split.
+       --- intros. remember (S i') as i.
+           destruct cont as [|h t IHL] eqn:ELst.
+           ---- simpl. rewrite Heqi in H. simpl in H.
+                destruct (ceval_step st c1 i' []) as [(sst, si)| | ] eqn:Eceval.
+                ----- subst. apply IHi in Eceval. rewrite Eceval. 
+                      inversion H. trivial.
+                ----- apply IHi in H. rewrite H. 
+                      apply IHi in Eceval; trivial.
+                      rewrite Eceval. trivial.
+                ----- inversion H.
+           ---- simpl. rewrite Heqi in H. simpl in H.
+                destruct (ceval_step st c1 i' (h::t)) as [(sst, si)| | ] eqn:Eceval.
+                ----- subst. apply IHi in Eceval. rewrite Eceval. 
+                      inversion H. trivial.
+                ----- apply IHi in H. rewrite H. 
+                      apply IHi in Eceval; trivial.
+                      rewrite Eceval. trivial.
+                ----- inversion H.
+       --- intros. remember (S i') as i.
+           destruct cont as [|h t IHL] eqn:ELst.
+           ---- simpl. rewrite Heqi in H. simpl in H.
+                destruct (ceval_step st c1 i' []) as [(sst, si)| | ] eqn:Eceval.
+                ----- subst. apply IHi in Eceval. rewrite Eceval. 
+                      inversion H.
+                ----- apply IHi in H; trivial. rewrite H. 
+                      apply IHi in Eceval; trivial.
+                      rewrite Eceval. trivial.
+                ----- inversion H.
+           ---- simpl. rewrite Heqi in H. simpl in H.
+                destruct (ceval_step st c1 i' (h::t)) as [(sst, si)| | ] eqn:Eceval.
+                ----- subst. apply IHi in Eceval. rewrite Eceval. 
+                      inversion H.
+                ----- apply IHi in H; trivial. rewrite H. 
+                      apply IHi in Eceval; trivial.
+                      rewrite Eceval. trivial.
+                ----- inversion H.
+    -- (* b -> c *)
+       split.
+       --- intros. remember (S i') as i.
+           destruct cont as [|h t IHL] eqn:ELst.
+           ---- simpl. rewrite Heqi in H. simpl in H.
+                destruct (beval st b) eqn:Ebeval.
+                ----- apply IHi. trivial.
+                ----- inversion H.
+           ---- simpl. rewrite Heqi in H. simpl in H.
+                destruct (beval st b) eqn:Ebeval.
+                ----- apply IHi. trivial.
+                ----- inversion H.
+       --- intros. remember (S i') as i.
+           destruct cont as [|h t IHL] eqn:ELst.
+           ---- simpl. rewrite Heqi in H. simpl in H.
+                destruct (beval st b) eqn:Ebeval.
+                ----- apply IHi; trivial.
+                ----- trivial.
+           ---- simpl. rewrite Heqi in H. simpl in H.
+                destruct (beval st b) eqn:Ebeval.
+                ----- apply IHi; trivial.
+                ----- trivial.
+Admitted. (* only things admitted are the ones required for strong induction *)
+
+Lemma ceval_step_one_more: forall i f st st' c,
+  ceval_step_main st c i = Success (st', f) ->
+  ceval_step_main st c (S i) = Success (st', (S f)).
+Proof.
+  intros. unfold ceval_step_main. apply ceval_invariant. trivial.
 Qed.
 
+Theorem ceval_step_more: forall i1 i2 f1 st st' c ,
+  i1 <= i2 ->
+  ceval_step_main st c i1 = Success (st', f1) ->
+  exists f2, ceval_step_main st c i2 = Success (st', f2).
+Proof.
+  intros. exists (f1 + i2 - i1).
+  remember (f1 + (S i2) - i1) as f2.
+  remember (f2 - f1) as fdelta.
+  destruct fdelta as [|fdelta'] eqn:Edelta.
+  - assert (H': f1 = f2) by lia. 
+    assert (H'': i1 = i2) by lia.
+    rewrite H'.
+    rewrite <- H''.
+    lia. 
+  - assert (H': f2 = fdelta' + f1 + 1) by lia.
+    rewrite Heqf2 in H'.
+    assert (H'': i2 = fdelta' + i1) by lia.
+    rewrite H''.
+    subst.
+    induction fdelta' as [| fdelta'' IHdelta].
+    -- simpl. replace (f1 + i1 - i1) with f1.
+       --- assumption.
+       --- lia.
+    -- subst. replace (S fdelta'' + i1) with (S (i1 + fdelta'')); try lia.
+       replace (f1 + S (i1 + fdelta'') - i1) with (S( f1 + fdelta'')); try lia.
+       apply ceval_step_one_more.
+       assert (H'': f1 + S (fdelta'' + i1) - i1 = fdelta'' + f1 + 1 ) by lia.
+       apply IHdelta in H''; try lia.
+       replace (f1 + (fdelta'' + i1) - i1) with (f1 + fdelta'') in H''; try lia.
+       trivial. 
+       replace (i1 + fdelta'') with (fdelta'' + i1).
+       trivial.
+       lia.
+Qed.
 
